program_logic/auth.v
@@ -2,53 +2,52 @@ From algebra Require Export auth.
 From program_logic Require Export invariants ghost_ownership.
 Import uPred.
 
-Class AuthInG Λ Σ (i : gid) (A : cmraT) `{Empty A} := {
-  auth_inG :> InG Λ Σ i (authRA A);
+(* TODO: Once we switched to RAs, it is no longer necessary to remember that a
+is constantly valid. *)
+Class authG Λ Σ (A : cmraT) `{Empty A} := AuthG {
+  auth_inG :> inG Λ Σ (authRA A);
   auth_identity :> CMRAIdentity A;
   auth_timeless (a : A) :> Timeless a;
 }.
 
-(* TODO: Once we switched to RAs, it is no longer necessary to remember that a is
-   constantly valid. *)
 Section definitions.
-  Context {Λ Σ A} (i : gid) `{AuthInG Λ Σ i A} (γ : gname).
+  Context `{authG Λ Σ A} (γ : gname).
   Definition auth_inv (φ : A → iPropG Λ Σ) : iPropG Λ Σ :=
-    (∃ a, (■ ✓ a ∧ own i γ (● a)) ★ φ a)%I.
-  Definition auth_own (a : A) : iPropG Λ Σ := own i γ (◯ a).
+    (∃ a, (■ ✓ a ∧ own γ (● a)) ★ φ a)%I.
+  Definition auth_own (a : A) : iPropG Λ Σ := own γ (◯ a).
   Definition auth_ctx (N : namespace) (φ : A → iPropG Λ Σ) : iPropG Λ Σ :=
     inv N (auth_inv φ).
 End definitions.
-Instance: Params (@auth_inv) 7.
-Instance: Params (@auth_own) 7.
-Instance: Params (@auth_ctx) 8.
+Instance: Params (@auth_inv) 6.
+Instance: Params (@auth_own) 6.
+Instance: Params (@auth_ctx) 7.
 
 Section auth.
-  Context `{AuthInG Λ Σ AuthI A}.
+  Context `{AuthI : authG Λ Σ A}.
   Context (φ : A → iPropG Λ Σ) {φ_proper : Proper ((≡) ==> (≡)) φ}.
   Implicit Types N : namespace.
   Implicit Types P Q R : iPropG Λ Σ.
   Implicit Types a b : A.
   Implicit Types γ : gname.
 
-  Global Instance auth_own_ne n γ :
-    Proper (dist n ==> dist n) (auth_own AuthI γ).
+  Global Instance auth_own_ne n γ : Proper (dist n ==> dist n) (auth_own γ).
   Proof. by rewrite /auth_own=> a b ->. Qed.
-  Global Instance auth_own_proper γ : Proper ((≡) ==> (≡)) (auth_own AuthI γ).
+  Global Instance auth_own_proper γ : Proper ((≡) ==> (≡)) (auth_own γ).
   Proof. by rewrite /auth_own=> a b ->. Qed.
   Lemma auto_own_op γ a b :
-    auth_own AuthI γ (a ⋅ b) ≡ (auth_own AuthI γ a ★ auth_own AuthI γ b)%I.
+    auth_own γ (a ⋅ b) ≡ (auth_own γ a ★ auth_own γ b)%I.
   Proof. by rewrite /auth_own -own_op auth_frag_op. Qed.
-  Lemma auto_own_valid γ a : auth_own AuthI γ a ⊑ ✓ a.
+  Lemma auto_own_valid γ a : auth_own γ a ⊑ ✓ a.
   Proof. by rewrite /auth_own own_valid auth_validI. Qed.
 
   Lemma auth_alloc N a :
-    ✓ a → φ a ⊑ pvs N N (∃ γ, auth_ctx AuthI γ N φ ∧ auth_own AuthI γ a).
+    ✓ a → φ a ⊑ pvs N N (∃ γ, auth_ctx γ N φ ∧ auth_own γ a).
   Proof.
     intros Ha. eapply sep_elim_True_r.
-    { by eapply (own_alloc AuthI (Auth (Excl a) a) N). }
+    { by eapply (own_alloc (Auth (Excl a) a) N). }
     rewrite pvs_frame_l. apply pvs_strip_pvs.
     rewrite sep_exist_l. apply exist_elim=>γ. rewrite -(exist_intro γ).
-    transitivity (▷ auth_inv AuthI γ φ ★ auth_own AuthI γ a)%I.
+    transitivity (▷ auth_inv γ φ ★ auth_own γ a)%I.
     { rewrite /auth_inv -later_intro -(exist_intro a).
       rewrite const_equiv // left_id.
       rewrite [(_ ★ φ _)%I]comm -assoc. apply sep_mono; first done.
@@ -57,12 +56,12 @@ Section auth.
     by rewrite always_and_sep_l.
   Qed.
 
-  Lemma auth_empty E γ : True ⊑ pvs E E (auth_own AuthI γ ∅).
-  Proof. by rewrite own_update_empty /auth_own. Qed.
+  Lemma auth_empty γ E : True ⊑ pvs E E (auth_own γ ∅).
+  Proof. by rewrite /auth_own -own_update_empty. Qed.
 
   Lemma auth_opened E γ a :
-    (▷ auth_inv AuthI γ φ ★ auth_own AuthI γ a)
-    ⊑ pvs E E (∃ a', ■ ✓ (a ⋅ a') ★ ▷ φ (a ⋅ a') ★ own AuthI γ (● (a ⋅ a') ⋅ ◯ a)).
+    (▷ auth_inv γ φ ★ auth_own γ a)
+    ⊑ pvs E E (∃ a', ■ ✓ (a ⋅ a') ★ ▷ φ (a ⋅ a') ★ own γ (● (a ⋅ a') ⋅ ◯ a)).
   Proof.
     rewrite /auth_inv. rewrite later_exist sep_exist_r. apply exist_elim=>b.
     rewrite later_sep [(▷(_ ∧ _))%I]pvs_timeless !pvs_frame_r. apply pvs_mono.
@@ -71,7 +70,7 @@ Section auth.
     rewrite own_valid_r auth_validI /= and_elim_l sep_exist_l sep_exist_r /=.
     apply exist_elim=>a'.
     rewrite left_id -(exist_intro a').
-    apply (eq_rewrite b (a ⋅ a') (λ x, ■✓x ★ ▷φ x ★ own AuthI γ (● x ⋅ ◯ a))%I).
+    apply (eq_rewrite b (a ⋅ a') (λ x, ■ ✓ x ★ ▷ φ x ★ own γ (● x ⋅ ◯ a))%I).
     { by move=>n ? ? /timeless_iff ->. }
     { by eauto with I. }
     rewrite const_equiv // left_id comm.
@@ -81,8 +80,8 @@ Section auth.
 
   Lemma auth_closing `{!LocalUpdate Lv L} E γ a a' :
     Lv a → ✓ (L a ⋅ a') →
-    (▷ φ (L a ⋅ a') ★ own AuthI γ (● (a ⋅ a') ⋅ ◯ a))
-    ⊑ pvs E E (▷ auth_inv AuthI γ φ ★ auth_own AuthI γ (L a)).
+    (▷ φ (L a ⋅ a') ★ own γ (● (a ⋅ a') ⋅ ◯ a))
+    ⊑ pvs E E (▷ auth_inv γ φ ★ auth_own γ (L a)).
   Proof.
     intros HL Hv. rewrite /auth_inv /auth_own -(exist_intro (L a ⋅ a')).
     rewrite later_sep [(_ ★ ▷φ _)%I]comm -assoc.
@@ -99,12 +98,12 @@ Section auth.
   Lemma auth_fsa E N P (Q : V → iPropG Λ Σ) γ a :
     fsaV →
     nclose N ⊆ E →
-    P ⊑ auth_ctx AuthI γ N φ →
-    P ⊑ (▷ auth_own AuthI γ a ★ ∀ a',
+    P ⊑ auth_ctx γ N φ →
+    P ⊑ (▷ auth_own γ a ★ ∀ a',
           ■ ✓ (a ⋅ a') ★ ▷ φ (a ⋅ a') -★
           fsa (E ∖ nclose N) (λ x, ∃ L Lv (Hup : LocalUpdate Lv L),
             ■ (Lv a ∧ ✓ (L a ⋅ a')) ★ ▷ φ (L a ⋅ a') ★
-            (auth_own AuthI γ (L a) -★ Q x))) →
+            (auth_own γ (L a) -★ Q x))) →
     P ⊑ fsa E Q.
   Proof.
     rewrite /auth_ctx=>? HN Hinv Hinner.
@@ -131,12 +130,12 @@ Section auth.
   Lemma auth_fsa' L `{!LocalUpdate Lv L} E N P (Q: V → iPropG Λ Σ) γ a :
     fsaV →
     nclose N ⊆ E →
-    P ⊑ auth_ctx AuthI γ N φ →
-    P ⊑ (▷ auth_own AuthI γ a ★ (∀ a',
+    P ⊑ auth_ctx γ N φ →
+    P ⊑ (▷ auth_own γ a ★ (∀ a',
           ■ ✓ (a ⋅ a') ★ ▷ φ (a ⋅ a') -★
           fsa (E ∖ nclose N) (λ x,
             ■ (Lv a ∧ ✓ (L a ⋅ a')) ★ ▷ φ (L a ⋅ a') ★
-            (auth_own AuthI γ (L a) -★ Q x)))) →
+            (auth_own γ (L a) -★ Q x)))) →
     P ⊑ fsa E Q.
   Proof.
     intros ??? HP. eapply auth_fsa with N γ a; eauto.
