program_logic/ghost_ownership.v
@@ -11,101 +11,103 @@ Definition gname := positive.
 Definition globalF (Σ : gid → iFunctor) : iFunctor :=
   iprodF (λ i, mapF gname (Σ i)).
 
-Class InG (Λ : language) (Σ : gid → iFunctor) (i : gid) (A : cmraT) :=
-  inG : A = Σ i (laterC (iPreProp Λ (globalF Σ))).
+Class inG (Λ : language) (Σ : gid → iFunctor) (A : cmraT) := InG {
+  inG_id : gid;
+  inG_prf : A = Σ inG_id (laterC (iPreProp Λ (globalF Σ)))
+}.
 
-Definition to_globalF {Λ Σ A}
-    (i : gid) `{!InG Λ Σ i A} (γ : gname) (a : A) : iGst Λ (globalF Σ) :=
-  iprod_singleton i {[ γ ↦ cmra_transport inG a ]}.
-Definition own {Λ Σ A}
-    (i : gid) `{!InG Λ Σ i A} (γ : gname) (a : A) : iProp Λ (globalF Σ) :=
-  ownG (to_globalF i γ a).
-Instance: Params (@to_globalF) 6.
-Instance: Params (@own) 6.
+Definition to_globalF `{inG Λ Σ A} (γ : gname) (a : A) : iGst Λ (globalF Σ) :=
+  iprod_singleton inG_id {[ γ ↦ cmra_transport inG_prf a ]}.
+Definition own `{inG Λ Σ A} (γ : gname) (a : A) : iProp Λ (globalF Σ) :=
+  ownG (to_globalF γ a).
+Instance: Params (@to_globalF) 5.
+Instance: Params (@own) 5.
 Typeclasses Opaque to_globalF own.
 
 Notation iPropG Λ Σ := (iProp Λ (globalF Σ)).
 Notation iFunctorG := (gid → iFunctor).
 
 Section global.
-Context {Λ : language} {Σ : iFunctorG} (i : gid) `{!InG Λ Σ i A}.
+Context `{i : inG Λ Σ A}.
 Implicit Types a : A.
 
 (** * Properties of to_globalC *)
-Instance to_globalF_ne γ n : Proper (dist n ==> dist n) (to_globalF i γ).
+Instance to_globalF_ne γ n : Proper (dist n ==> dist n) (to_globalF γ).
 Proof. by intros a a' Ha; apply iprod_singleton_ne; rewrite Ha. Qed.
 Lemma to_globalF_op γ a1 a2 :
-  to_globalF i γ (a1 ⋅ a2) ≡ to_globalF i γ a1 ⋅ to_globalF i γ a2.
+  to_globalF γ (a1 ⋅ a2) ≡ to_globalF γ a1 ⋅ to_globalF γ a2.
 Proof.
   by rewrite /to_globalF iprod_op_singleton map_op_singleton cmra_transport_op.
 Qed.
-Lemma to_globalF_unit γ a : unit (to_globalF i γ a) ≡ to_globalF i γ (unit a).
+Lemma to_globalF_unit γ a : unit (to_globalF γ a) ≡ to_globalF γ (unit a).
 Proof.
   by rewrite /to_globalF
     iprod_unit_singleton map_unit_singleton cmra_transport_unit.
 Qed.
-Instance to_globalF_timeless γ m : Timeless m → Timeless (to_globalF i γ m).
+Instance to_globalF_timeless γ m : Timeless m → Timeless (to_globalF γ m).
 Proof. rewrite /to_globalF; apply _. Qed.
 
 (** * Transport empty *)
-Instance inG_empty `{Empty A} : Empty (Σ i (laterC (iPreProp Λ (globalF Σ)))) :=
-  cmra_transport inG ∅.
+Instance inG_empty `{Empty A} :
+  Empty (Σ inG_id (laterC (iPreProp Λ (globalF Σ)))) := cmra_transport inG_prf ∅.
 Instance inG_empty_spec `{Empty A} :
-  CMRAIdentity A → CMRAIdentity (Σ i (laterC (iPreProp Λ (globalF Σ)))).
+  CMRAIdentity A → CMRAIdentity (Σ inG_id (laterC (iPreProp Λ (globalF Σ)))).
 Proof.
   split.
   * apply cmra_transport_valid, cmra_empty_valid.
-  * intros x; rewrite /empty /inG_empty; destruct inG. by rewrite left_id.
+  * intros x; rewrite /empty /inG_empty; destruct inG_prf. by rewrite left_id.
   * apply _.
 Qed.
 
 (** * Properties of own *)
-Global Instance own_ne γ n : Proper (dist n ==> dist n) (own i γ).
+Global Instance own_ne γ n : Proper (dist n ==> dist n) (own γ).
 Proof. by intros m m' Hm; rewrite /own Hm. Qed.
-Global Instance own_proper γ : Proper ((≡) ==> (≡)) (own i γ) := ne_proper _.
+Global Instance own_proper γ : Proper ((≡) ==> (≡)) (own γ) := ne_proper _.
 
-Lemma own_op γ a1 a2 : own i γ (a1 ⋅ a2) ≡ (own i γ a1 ★ own i γ a2)%I.
+Lemma own_op γ a1 a2 : own γ (a1 ⋅ a2) ≡ (own γ a1 ★ own γ a2)%I.
 Proof. by rewrite /own -ownG_op to_globalF_op. Qed.
-Global Instance own_mono γ : Proper (flip (≼) ==> (⊑)) (own i γ).
+Global Instance own_mono γ : Proper (flip (≼) ==> (⊑)) (own γ).
 Proof. move=>a b [c H]. rewrite H own_op. eauto with I. Qed.
-Lemma always_own_unit γ a : (□ own i γ (unit a))%I ≡ own i γ (unit a).
+Lemma always_own_unit γ a : (□ own γ (unit a))%I ≡ own γ (unit a).
 Proof. by rewrite /own -to_globalF_unit always_ownG_unit. Qed.
-Lemma own_valid γ a : own i γ a ⊑ ✓ a.
+Lemma own_valid γ a : own γ a ⊑ ✓ a.
 Proof.
   rewrite /own ownG_valid /to_globalF.
-  rewrite iprod_validI (forall_elim i) iprod_lookup_singleton.
+  rewrite iprod_validI (forall_elim inG_id) iprod_lookup_singleton.
   rewrite map_validI (forall_elim γ) lookup_singleton option_validI.
-  by destruct inG.
+  by destruct inG_prf.
 Qed.
-Lemma own_valid_r γ a : own i γ a ⊑ (own i γ a ★ ✓ a).
+Lemma own_valid_r γ a : own γ a ⊑ (own γ a ★ ✓ a).
 Proof. apply (uPred.always_entails_r _ _), own_valid. Qed.
-Lemma own_valid_l γ a : own i γ a ⊑ (✓ a ★ own i γ a).
+Lemma own_valid_l γ a : own γ a ⊑ (✓ a ★ own γ a).
 Proof. by rewrite comm -own_valid_r. Qed.
-Global Instance own_timeless γ a : Timeless a → TimelessP (own i γ a).
+Global Instance own_timeless γ a : Timeless a → TimelessP (own γ a).
 Proof. unfold own; apply _. Qed.
 
 (* TODO: This also holds if we just have ✓ a at the current step-idx, as Iris
    assertion. However, the map_updateP_alloc does not suffice to show this. *)
-Lemma own_alloc_strong a E (G : gset gname) : ✓ a → True ⊑ pvs E E (∃ γ, ■(γ ∉ G) ∧ own i γ a).
+Lemma own_alloc_strong a E (G : gset gname) :
+  ✓ a → True ⊑ pvs E E (∃ γ, ■(γ ∉ G) ∧ own γ a).
 Proof.
   intros Ha.
-  rewrite -(pvs_mono _ _ (∃ m, ■ (∃ γ, γ ∉ G ∧ m = to_globalF i γ a) ∧ ownG m)%I).
-  * eapply pvs_ownG_updateP_empty, (iprod_singleton_updateP_empty i);
-      first (eapply map_updateP_alloc_strong', cmra_transport_valid, Ha); naive_solver.
+  rewrite -(pvs_mono _ _ (∃ m, ■ (∃ γ, γ ∉ G ∧ m = to_globalF γ a) ∧ ownG m)%I).
+  * eapply pvs_ownG_updateP_empty, (iprod_singleton_updateP_empty inG_id);
+      first (eapply map_updateP_alloc_strong', cmra_transport_valid, Ha);
+      naive_solver.
   * apply exist_elim=>m; apply const_elim_l=>-[γ [Hfresh ->]].
     by rewrite -(exist_intro γ) const_equiv.
 Qed.
-Lemma own_alloc a E : ✓ a → True ⊑ pvs E E (∃ γ, own i γ a).
+Lemma own_alloc a E : ✓ a → True ⊑ pvs E E (∃ γ, own γ a).
 Proof.
   intros Ha. rewrite (own_alloc_strong a E ∅) //; []. apply pvs_mono.
   apply exist_mono=>?. eauto with I.
 Qed.
 
 Lemma own_updateP P γ a E :
-  a ~~>: P → own i γ a ⊑ pvs E E (∃ a', ■ P a' ∧ own i γ a').
+  a ~~>: P → own γ a ⊑ pvs E E (∃ a', ■ P a' ∧ own γ a').
 Proof.
   intros Ha.
-  rewrite -(pvs_mono _ _ (∃ m, ■ (∃ a', m = to_globalF i γ a' ∧ P a') ∧ ownG m)%I).
+  rewrite -(pvs_mono _ _ (∃ m, ■ (∃ a', m = to_globalF γ a' ∧ P a') ∧ ownG m)%I).
   * eapply pvs_ownG_updateP, iprod_singleton_updateP;
       first by (eapply map_singleton_updateP', cmra_transport_updateP', Ha).
     naive_solver.
@@ -114,10 +116,10 @@ Proof.
 Qed.
 
 Lemma own_updateP_empty `{Empty A, !CMRAIdentity A} P γ E :
-  ∅ ~~>: P → True ⊑ pvs E E (∃ a, ■ P a ∧ own i γ a).
+  ∅ ~~>: P → True ⊑ pvs E E (∃ a, ■ P a ∧ own γ a).
 Proof.
   intros Hemp.
-  rewrite -(pvs_mono _ _ (∃ m, ■ (∃ a', m = to_globalF i γ a' ∧ P a') ∧ ownG m)%I).
+  rewrite -(pvs_mono _ _ (∃ m, ■ (∃ a', m = to_globalF γ a' ∧ P a') ∧ ownG m)%I).
   * eapply pvs_ownG_updateP_empty, iprod_singleton_updateP_empty;
       first eapply map_singleton_updateP_empty', cmra_transport_updateP', Hemp.
     naive_solver.
@@ -125,14 +127,14 @@ Proof.
     rewrite -(exist_intro a'). by apply and_intro; [apply const_intro|].
 Qed.
 
-Lemma own_update γ a a' E : a ~~> a' → own i γ a ⊑ pvs E E (own i γ a').
+Lemma own_update γ a a' E : a ~~> a' → own γ a ⊑ pvs E E (own γ a').
 Proof.
   intros; rewrite (own_updateP (a' =)); last by apply cmra_update_updateP.
   by apply pvs_mono, exist_elim=> a''; apply const_elim_l=> ->.
 Qed.
 
 Lemma own_update_empty `{Empty A, !CMRAIdentity A} γ E :
-  True ⊑ pvs E E (own i γ ∅).
+  True ⊑ pvs E E (own γ ∅).
 Proof.
   rewrite (own_updateP_empty (∅ =)); last by apply cmra_updateP_id.
   apply pvs_mono, exist_elim=>a. by apply const_elim_l=>->.
