program_logic/saved_prop.v
@@ -2,29 +2,29 @@ From algebra Require Export agree.
 From program_logic Require Export ghost_ownership.
 Import uPred.
 
-Class SavedPropInG Λ Σ (i : gid) :=
-  saved_prop_inG :> InG Λ Σ i (agreeRA (laterC (iPreProp Λ (globalF Σ)))).
+Notation savedPropG Λ Σ :=
+  (inG Λ Σ (agreeRA (laterC (iPreProp Λ (globalF Σ))))).
 
-Definition saved_prop_own {Λ Σ} (i : gid) `{SavedPropInG Λ Σ i}
+Definition saved_prop_own `{savedPropG Λ Σ}
     (γ : gname) (P : iPropG Λ Σ) : iPropG Λ Σ :=
-  own i γ (to_agree (Next (iProp_unfold P))).
-Instance: Params (@saved_prop_own) 5.
+  own γ (to_agree (Next (iProp_unfold P))).
+Instance: Params (@saved_prop_own) 4.
 
 Section saved_prop.
-  Context `{SavedPropInG Λ Σ SPI}.
+  Context `{savedPropG Λ Σ}.
   Implicit Types P Q : iPropG Λ Σ.
   Implicit Types γ : gname.
 
   Lemma saved_prop_alloc_strong N P (G : gset gname) :
-    True ⊑ pvs N N (∃ γ, ■ (γ ∉ G) ∧ saved_prop_own SPI γ P).
+    True ⊑ pvs N N (∃ γ, ■ (γ ∉ G) ∧ saved_prop_own γ P).
   Proof. by apply own_alloc_strong. Qed.
 
   Lemma saved_prop_alloc N P :
-    True ⊑ pvs N N (∃ γ, saved_prop_own SPI γ P).
+    True ⊑ pvs N N (∃ γ, saved_prop_own γ P).
   Proof. by apply own_alloc. Qed.
 
   Lemma saved_prop_agree γ P Q :
-    (saved_prop_own SPI γ P ★ saved_prop_own SPI γ Q) ⊑ ▷ (P ≡ Q).
+    (saved_prop_own γ P ★ saved_prop_own γ Q) ⊑ ▷ (P ≡ Q).
   Proof.
     rewrite /saved_prop_own -own_op own_valid agree_validI.
     rewrite agree_equivI later_equivI /=; apply later_mono.
