program_logic/sts.v
@@ -2,31 +2,31 @@ From algebra Require Export sts.
 From program_logic Require Export invariants ghost_ownership.
 Import uPred.
 
-Class STSInG Λ Σ (i : gid) (sts : stsT) := {
-  sts_inG :> ghost_ownership.InG Λ Σ i (stsRA sts);
+Class stsG Λ Σ (sts : stsT) := StsG {
+  sts_inG :> inG Λ Σ (stsRA sts);
   sts_inhabited :> Inhabited (sts.state sts);
 }.
+Coercion sts_inG : stsG >-> inG.
 
 Section definitions.
-  Context {Λ Σ} (i : gid) (sts : stsT) `{!STSInG Λ Σ i sts} (γ : gname).
+  Context `{i : stsG Λ Σ sts} (γ : gname).
   Import sts.
   Definition sts_inv (φ : state sts → iPropG Λ Σ) : iPropG Λ Σ :=
-    (∃ s, own i γ (sts_auth s ∅) ★ φ s)%I.
+    (∃ s, own γ (sts_auth s ∅) ★ φ s)%I.
   Definition sts_ownS (S : states sts) (T : tokens sts) : iPropG Λ Σ:=
-    own i γ (sts_frag S T).
+    own γ (sts_frag S T).
   Definition sts_own (s : state sts) (T : tokens sts) : iPropG Λ Σ :=
-    own i γ (sts_frag_up s T).
+    own γ (sts_frag_up s T).
   Definition sts_ctx (N : namespace) (φ: state sts → iPropG Λ Σ) : iPropG Λ Σ :=
     inv N (sts_inv φ).
 End definitions.
-Instance: Params (@sts_inv) 6.
-Instance: Params (@sts_ownS) 6.
-Instance: Params (@sts_own) 7.
-Instance: Params (@sts_ctx) 7.
+Instance: Params (@sts_inv) 5.
+Instance: Params (@sts_ownS) 5.
+Instance: Params (@sts_own) 6.
+Instance: Params (@sts_ctx) 6.
 
 Section sts.
-  Context {Λ Σ} (i : gid) (sts : stsT) `{!STSInG Λ Σ StsI sts}.
-  Context (φ : sts.state sts → iPropG Λ Σ).
+  Context `{stsG Λ Σ sts} (φ : sts.state sts → iPropG Λ Σ).
   Implicit Types N : namespace.
   Implicit Types P Q R : iPropG Λ Σ.
   Implicit Types γ : gname.
@@ -35,57 +35,55 @@ Section sts.
 
   (** Setoids *)
   Global Instance sts_inv_ne n γ :
-    Proper (pointwise_relation _ (dist n) ==> dist n) (sts_inv StsI sts γ).
+    Proper (pointwise_relation _ (dist n) ==> dist n) (sts_inv γ).
   Proof. by intros φ1 φ2 Hφ; rewrite /sts_inv; setoid_rewrite Hφ. Qed.
   Global Instance sts_inv_proper γ :
-    Proper (pointwise_relation _ (≡) ==> (≡)) (sts_inv StsI sts γ).
+    Proper (pointwise_relation _ (≡) ==> (≡)) (sts_inv γ).
   Proof. by intros φ1 φ2 Hφ; rewrite /sts_inv; setoid_rewrite Hφ. Qed.
-  Global Instance sts_ownS_proper γ :
-    Proper ((≡) ==> (≡) ==> (≡)) (sts_ownS StsI sts γ).
+  Global Instance sts_ownS_proper γ : Proper ((≡) ==> (≡) ==> (≡)) (sts_ownS γ).
   Proof. intros S1 S2 HS T1 T2 HT. by rewrite /sts_ownS HS HT. Qed.
-  Global Instance sts_own_proper γ s :
-    Proper ((≡) ==> (≡)) (sts_ownS StsI sts γ s).
+  Global Instance sts_own_proper γ s : Proper ((≡) ==> (≡)) (sts_ownS γ s).
   Proof. intros T1 T2 HT. by rewrite /sts_ownS HT. Qed.
   Global Instance sts_ctx_ne n γ N :
-    Proper (pointwise_relation _ (dist n) ==> dist n) (sts_ctx StsI sts γ N).
+    Proper (pointwise_relation _ (dist n) ==> dist n) (sts_ctx γ N).
   Proof. by intros φ1 φ2 Hφ; rewrite /sts_ctx Hφ. Qed.
   Global Instance sts_ctx_proper γ N :
-    Proper (pointwise_relation _ (≡) ==> (≡)) (sts_ctx StsI sts γ N).
+    Proper (pointwise_relation _ (≡) ==> (≡)) (sts_ctx γ N).
   Proof. by intros φ1 φ2 Hφ; rewrite /sts_ctx Hφ. Qed.
 
   (* The same rule as implication does *not* hold, as could be shown using
      sts_frag_included. *)
   Lemma sts_ownS_weaken E γ S1 S2 T :
     S1 ⊆ S2 → sts.closed S2 T →
-    sts_ownS StsI sts γ S1 T ⊑ pvs E E (sts_ownS StsI sts γ S2 T).
+    sts_ownS γ S1 T ⊑ pvs E E (sts_ownS γ S2 T).
   Proof. intros. by apply own_update, sts_update_frag. Qed.
 
   Lemma sts_own_weaken E γ s S T :
     s ∈ S → sts.closed S T →
-    sts_own StsI sts γ s T ⊑ pvs E E (sts_ownS StsI sts γ S T).
+    sts_own γ s T ⊑ pvs E E (sts_ownS γ S T).
   Proof. intros. by apply own_update, sts_update_frag_up. Qed.
 
   Lemma sts_alloc N s :
-    φ s ⊑ pvs N N (∃ γ, sts_ctx StsI sts γ N φ ∧
-                        sts_own StsI sts γ s (set_all ∖ sts.tok s)).
+    φ s ⊑ pvs N N (∃ γ, sts_ctx γ N φ ∧
+                        sts_own γ s (set_all ∖ sts.tok s)).
   Proof.
     eapply sep_elim_True_r.
-    { apply (own_alloc StsI (sts_auth s (set_all ∖ sts.tok s)) N).
+    { apply (own_alloc (sts_auth s (set_all ∖ sts.tok s)) N).
       apply sts_auth_valid; solve_elem_of. }
     rewrite pvs_frame_l. apply pvs_strip_pvs.
     rewrite sep_exist_l. apply exist_elim=>γ. rewrite -(exist_intro γ).
-    transitivity (▷ sts_inv StsI sts γ φ ★
-                    sts_own StsI sts γ s (set_all ∖ sts.tok s))%I.
+    transitivity (▷ sts_inv γ φ ★
+                    sts_own γ s (set_all ∖ sts.tok s))%I.
     { rewrite /sts_inv -later_intro -(exist_intro s).
       rewrite [(_ ★ φ _)%I]comm -assoc. apply sep_mono_r.
-      by rewrite -own_op sts_op_auth_frag_up; last solve_elem_of+. }
+      by rewrite -own_op sts_op_auth_frag_up; last solve_elem_of. }
     rewrite (inv_alloc N) /sts_ctx pvs_frame_r.
     by rewrite always_and_sep_l.
   Qed.
 
   Lemma sts_opened E γ S T :
-    (▷ sts_inv StsI sts γ φ ★ sts_ownS StsI sts γ S T)
-    ⊑ pvs E E (∃ s, ■ (s ∈ S) ★ ▷ φ s ★ own StsI γ (sts_auth s T)).
+    (▷ sts_inv γ φ ★ sts_ownS γ S T)
+    ⊑ pvs E E (∃ s, ■ (s ∈ S) ★ ▷ φ s ★ own γ (sts_auth s T)).
   Proof.
     rewrite /sts_inv /sts_ownS later_exist sep_exist_r. apply exist_elim=>s.
     rewrite later_sep pvs_timeless !pvs_frame_r. apply pvs_mono.
@@ -101,14 +99,13 @@ Section sts.
 
   Lemma sts_closing E γ s T s' T' :
     sts.step (s, T) (s', T') →
-    (▷ φ s' ★ own StsI γ (sts_auth s T))
-    ⊑ pvs E E (▷ sts_inv StsI sts γ φ ★ sts_own StsI sts γ s' T').
+    (▷ φ s' ★ own γ (sts_auth s T)) ⊑ pvs E E (▷ sts_inv γ φ ★ sts_own γ s' T').
   Proof.
     intros Hstep. rewrite /sts_inv /sts_own -(exist_intro s').
     rewrite later_sep [(_ ★ ▷φ _)%I]comm -assoc.
     rewrite -pvs_frame_l. apply sep_mono_r. rewrite -later_intro.
     rewrite own_valid_l discrete_validI. apply const_elim_sep_l=>Hval.
-    transitivity (pvs E E (own StsI γ (sts_auth s' T'))).
+    transitivity (pvs E E (own γ (sts_auth s' T'))).
     { by apply own_update, sts_update_auth. }
     by rewrite -own_op sts_op_auth_frag_up; last by inversion_clear Hstep.
   Qed.
@@ -117,12 +114,12 @@ Section sts.
 
   Lemma sts_fsaS E N P (Q : V → iPropG Λ Σ) γ S T :
     fsaV → nclose N ⊆ E →
-    P ⊑ sts_ctx StsI sts γ N φ →
-    P ⊑ (sts_ownS StsI sts γ S T ★ ∀ s,
+    P ⊑ sts_ctx γ N φ →
+    P ⊑ (sts_ownS γ S T ★ ∀ s,
           ■ (s ∈ S) ★ ▷ φ s -★
           fsa (E ∖ nclose N) (λ x, ∃ s' T',
             ■ sts.step (s, T) (s', T') ★ ▷ φ s' ★
-            (sts_own StsI sts γ s' T' -★ Q x))) →
+            (sts_own γ s' T' -★ Q x))) →
     P ⊑ fsa E Q.
   Proof.
     rewrite /sts_ctx=>? HN Hinv Hinner.
@@ -146,12 +143,12 @@ Section sts.
 
   Lemma sts_fsa E N P (Q : V → iPropG Λ Σ) γ s0 T :
     fsaV → nclose N ⊆ E →
-    P ⊑ sts_ctx StsI sts γ N φ →
-    P ⊑ (sts_own StsI sts γ s0 T ★ ∀ s,
+    P ⊑ sts_ctx γ N φ →
+    P ⊑ (sts_own γ s0 T ★ ∀ s,
           ■ (s ∈ sts.up s0 T) ★ ▷ φ s -★
           fsa (E ∖ nclose N) (λ x, ∃ s' T',
             ■ (sts.step (s, T) (s', T')) ★ ▷ φ s' ★
-            (sts_own StsI sts γ s' T' -★ Q x))) →
+            (sts_own γ s' T' -★ Q x))) →
     P ⊑ fsa E Q.
   Proof. apply sts_fsaS. Qed.
 End sts.
